@prefix dct:   <http://purl.org/dc/terms/> .
@prefix owl:   <http://www.w3.org/2002/07/owl#> .
@prefix rdf:   <http://www.w3.org/1999/02/22-rdf-syntax-ns#> .
@prefix skos:  <http://www.w3.org/2004/02/skos/core#> .
@prefix rdfs:  <http://www.w3.org/2000/01/rdf-schema#> .

skos:narrowerTransitive
        a                   rdf:Property , owl:TransitiveProperty , owl:ObjectProperty ;
        rdfs:isDefinedBy    <http://www.w3.org/2004/02/skos/core> ;
        rdfs:label          "has narrower transitive"@en ;
        rdfs:subPropertyOf  skos:semanticRelation ;
        owl:inverseOf       skos:broaderTransitive ;
        skos:definition     "\nskos:narrowerTransitive is a transitive superproperty of skos:narrower.\n" ;
        skos:scopeNote      "\nBy convention, skos:narrowerTransitive is not used to make assertions. Rather, the properties can be used to draw inferences about the transitive closure of the hierarchical relation, which is useful e.g. when implementing a simple query expansion algorithm in a search application.\n"@en .

skos:scopeNote  a           rdf:Property , owl:AnnotationProperty ;
        rdfs:isDefinedBy    <http://www.w3.org/2004/02/skos/core> ;
        rdfs:label          "scope note"@en ;
        rdfs:subPropertyOf  skos:note ;
        skos:definition     "\nA note that helps to clarify the meaning and/or the use of a concept.\n"@en .

skos:closeMatch  a          rdf:Property , owl:SymmetricProperty , owl:ObjectProperty ;
        rdfs:isDefinedBy    <http://www.w3.org/2004/02/skos/core> ;
        rdfs:label          "has close match"@en ;
        rdfs:subPropertyOf  skos:mappingRelation ;
        skos:definition     "\nskos:closeMatch is used to link two concepts that are sufficiently similar that they can be used interchangeably in some information retrieval applications. In order to avoid the possibility of \"compound errors\" when combining mappings across more than two concept schemes, skos:closeMatch is not declared to be a transitive property.\n"@en .

skos:Concept  a           owl:Class ;
        rdfs:isDefinedBy  <http://www.w3.org/2004/02/skos/core> ;
        rdfs:label        "Concept"@en ;
        skos:definition   "An idea or notion; a unit of thought."@en .

skos:inScheme  a          rdf:Property , owl:ObjectProperty ;
        rdfs:isDefinedBy  <http://www.w3.org/2004/02/skos/core> ;
        rdfs:label        "is in scheme"@en ;
        rdfs:range        skos:ConceptScheme ;
        skos:definition   "\nRelates a resource (for example a concept) to a concept scheme in which it is included.\n"@en ;
        skos:scopeNote    "\nA concept may be a member of more than one concept scheme.\n"@en .

skos:relatedMatch  a        rdf:Property , owl:SymmetricProperty , owl:ObjectProperty ;
        rdfs:isDefinedBy    <http://www.w3.org/2004/02/skos/core> ;
        rdfs:label          "has related match"@en ;
        rdfs:subPropertyOf  skos:related , skos:mappingRelation ;
        skos:definition     "\nskos:relatedMatch is used to state an associative mapping link between two conceptual resources in different concept schemes.\n"@en .

skos:related  a             rdf:Property , owl:SymmetricProperty , owl:ObjectProperty ;
        rdfs:comment        "\nskos:related is disjoint with skos:broaderTransitive\n"@en ;
        rdfs:isDefinedBy    <http://www.w3.org/2004/02/skos/core> ;
        rdfs:label          "has related"@en ;
        rdfs:subPropertyOf  skos:semanticRelation ;
        skos:definition     "\nRelates a concept to a concept with which there is an associative semantic relationship.\n"@en .

skos:ConceptScheme  a     owl:Class ;
        rdfs:isDefinedBy  <http://www.w3.org/2004/02/skos/core> ;
        rdfs:label        "Concept Scheme"@en ;
        owl:disjointWith  skos:Concept ;
        skos:definition   "\nA set of concepts, optionally including statements about semantic relationships between those concepts.\n"@en ;
        skos:example      "\nThesauri, classification schemes, subject heading lists, taxonomies, 'folksonomies', and other types of controlled vocabulary are all examples of concept schemes. Concept schemes are also embedded in glossaries and terminologies.\n"@en ;
        skos:scopeNote    "\nA concept scheme may be defined to include concepts from different sources.\n"@en .

skos:topConceptOf  a        rdf:Property , owl:ObjectProperty ;
        rdfs:domain         skos:Concept ;
        rdfs:isDefinedBy    <http://www.w3.org/2004/02/skos/core> ;
        rdfs:label          "is top concept in scheme"@en ;
        rdfs:range          skos:ConceptScheme ;
        rdfs:subPropertyOf  skos:inScheme ;
        owl:inverseOf       skos:hasTopConcept ;
        skos:definition     "\nRelates a concept to the concept scheme that it is a top level concept of.\n"@en .

skos:member  a            rdf:Property , owl:ObjectProperty ;
        rdfs:domain       skos:Collection ;
        rdfs:isDefinedBy  <http://www.w3.org/2004/02/skos/core> ;
        rdfs:label        "has member"@en ;
        rdfs:range        [ a            owl:Class ;
                            owl:unionOf  ( skos:Concept skos:Collection )
                          ] ;
        skos:definition   "Relates a collection to one of its members."@en .

skos:broadMatch  a          rdf:Property , owl:ObjectProperty ;
        rdfs:isDefinedBy    <http://www.w3.org/2004/02/skos/core> ;
        rdfs:label          "has broader match"@en ;
        rdfs:subPropertyOf  skos:broader , skos:mappingRelation ;
        owl:inverseOf       skos:narrowMatch ;
        skos:definition     "\nskos:broadMatch is used to state a hierarchical mapping link between two conceptual resources in different concept schemes.\n"@en .

skos:changeNote  a          rdf:Property , owl:AnnotationProperty ;
        rdfs:isDefinedBy    <http://www.w3.org/2004/02/skos/core> ;
        rdfs:label          "change note"@en ;
        rdfs:subPropertyOf  skos:note ;
        skos:definition     "A note about a modification to a concept."@en .

skos:definition  a          rdf:Property , owl:AnnotationProperty ;
        rdfs:isDefinedBy    <http://www.w3.org/2004/02/skos/core> ;
        rdfs:label          "definition"@en ;
        rdfs:subPropertyOf  skos:note ;
        skos:definition     "\nA statement or formal explanation of the meaning of a concept.\n"@en .

skos:editorialNote  a       rdf:Property , owl:AnnotationProperty ;
        rdfs:isDefinedBy    <http://www.w3.org/2004/02/skos/core> ;
        rdfs:label          "editorial note"@en ;
        rdfs:subPropertyOf  skos:note ;
        skos:definition     "\nA note for an editor, translator or maintainer of the vocabulary.\n"@en .

skos:example  a             rdf:Property , owl:AnnotationProperty ;
        rdfs:isDefinedBy    <http://www.w3.org/2004/02/skos/core> ;
        rdfs:label          "example"@en ;
        rdfs:subPropertyOf  skos:note ;
        skos:definition     "An example of the use of a concept."@en .

skos:historyNote  a         rdf:Property , owl:AnnotationProperty ;
        rdfs:isDefinedBy    <http://www.w3.org/2004/02/skos/core> ;
        rdfs:label          "history note"@en ;
        rdfs:subPropertyOf  skos:note ;
        skos:definition     "\nA note about the past state/use/meaning of a concept.\n"@en .

skos:exactMatch  a          rdf:Property , owl:TransitiveProperty , owl:SymmetricProperty , owl:ObjectProperty ;
        rdfs:comment        "\nskos:exactMatch is disjoint with each of the properties skos:broadMatch and skos:relatedMatch.\n"@en ;
        rdfs:isDefinedBy    <http://www.w3.org/2004/02/skos/core> ;
        rdfs:label          "has exact match"@en ;
        rdfs:subPropertyOf  skos:closeMatch ;
        skos:definition     "\nskos:exactMatch is used to link two concepts, indicating a high degree of confidence that the concepts can be used interchangeably across a wide range of information retrieval applications. skos:exactMatch is a transitive property, and is a sub-property of skos:closeMatch.\n"@en .

skos:prefLabel  a           rdf:Property , owl:AnnotationProperty ;
        rdfs:comment        "\nskos:prefLabel, skos:altLabel and skos:hiddenLabel are pairwise disjoint properties.\n"@en , "\nThe range of skos:prefLabel is the class of RDF plain literals.\n"@en , "\nA resource has no more than one value of skos:prefLabel per language tag, and no more than one value of skos:prefLabel without language tag.\n"@en ;
        rdfs:isDefinedBy    <http://www.w3.org/2004/02/skos/core> ;
        rdfs:label          "preferred label"@en ;
        rdfs:subPropertyOf  rdfs:label ;
        skos:definition     "\nThe preferred lexical label for a resource, in a given language.\n"@en .

skos:memberList  a        rdf:Property , owl:FunctionalProperty , owl:ObjectProperty ;
        rdfs:comment      "\nFor any resource, every item in the list given as the value of the skos:memberList property is also a value of the skos:member property.\n"@en ;
        rdfs:domain       skos:OrderedCollection ;
        rdfs:isDefinedBy  <http://www.w3.org/2004/02/skos/core> ;
        rdfs:label        "has member list"@en ;
        rdfs:range        rdf:List ;
        skos:definition   "\nRelates an ordered collection to the RDF list containing its members.\n"@en .

skos:notation  a          rdf:Property , owl:DatatypeProperty ;
        rdfs:isDefinedBy  <http://www.w3.org/2004/02/skos/core> ;
        rdfs:label        "notation"@en ;
        skos:definition   "\nA notation, also known as classification code, is a string of characters such as \"T58.5\" or \"303.4833\" used to uniquely identify a concept within the scope of a given concept scheme.\n"@en ;
        skos:scopeNote    "\nBy convention, skos:notation is used with a typed literal in the object position of the triple.\n"@en .

skos:altLabel  a            rdf:Property , owl:AnnotationProperty ;
        rdfs:comment        "\nskos:prefLabel, skos:altLabel and skos:hiddenLabel are pairwise disjoint properties.\n"@en , "\nThe range of skos:altLabel is the class of RDF plain literals.\n"@en ;
        rdfs:isDefinedBy    <http://www.w3.org/2004/02/skos/core> ;
        rdfs:label          "alternative label"@en ;
        rdfs:subPropertyOf  rdfs:label ;
        skos:definition     "An alternative lexical label for a resource."@en ;
        skos:example        "\nAcronyms, abbreviations, spelling variants, and irregular plural/singular forms may be included among the alternative labels for a concept. Mis-spelled terms are normally included as hidden labels (see skos:hiddenLabel).\n"@en .

skos:broaderTransitive
        a                   rdf:Property , owl:TransitiveProperty , owl:ObjectProperty ;
        rdfs:isDefinedBy    <http://www.w3.org/2004/02/skos/core> ;
        rdfs:label          "has broader transitive"@en ;
        rdfs:subPropertyOf  skos:semanticRelation ;
        owl:inverseOf       skos:narrowerTransitive ;
        skos:definition     "\nskos:broaderTransitive is a transitive superproperty of skos:broader.\n" ;
        skos:scopeNote      "\nBy convention, skos:broaderTransitive is not used to make assertions. Rather, the properties can be used to draw inferences about the transitive closure of the hierarchical relation, which is useful e.g. when implementing a simple query expansion algorithm in a search application.\n"@en .

skos:broader  a             rdf:Property , owl:ObjectProperty ;
        rdfs:comment        "\nBroader concepts are typically rendered as parents in a concept hierarchy (tree).\n"@en ;
        rdfs:isDefinedBy    <http://www.w3.org/2004/02/skos/core> ;
        rdfs:label          "has broader"@en ;
        rdfs:subPropertyOf  skos:broaderTransitive ;
        owl:inverseOf       skos:narrower ;
        skos:definition     "\nRelates a concept to a concept that is more general in meaning.\n"@en ;
        skos:scopeNote      "\nBy convention, skos:broader is only used to assert an immediate (i.e. direct) hierarchical link between two conceptual resources.\n"@en .

skos:mappingRelation  a     rdf:Property , owl:ObjectProperty ;
        rdfs:comment        "\nThese concept mapping relations mirror semantic relations, and the data model defined below is similar (with the exception of skos:exactMatch) to the data model defined for semantic relations. A distinct vocabulary is provided for concept mapping relations, to provide a convenient way to differentiate links within a concept scheme from links between concept schemes. However, this pattern of usage is not a formal requirement of the SKOS data model, and relies on informal definitions of best practice.\n"@en ;
        rdfs:isDefinedBy    <http://www.w3.org/2004/02/skos/core> ;
        rdfs:label          "is in mapping relation with"@en ;
        rdfs:subPropertyOf  skos:semanticRelation ;
        skos:definition     "\nRelates two concepts coming, by convention, from different schemes, and that have comparable meanings\n"@en .

skos:hasTopConcept  a     rdf:Property , owl:ObjectProperty ;
        rdfs:domain       skos:ConceptScheme ;
        rdfs:isDefinedBy  <http://www.w3.org/2004/02/skos/core> ;
        rdfs:label        "has top concept"@en ;
        rdfs:range        skos:Concept ;
        owl:inverseOf     skos:topConceptOf ;
        skos:definition   "\nRelates, by convention, a concept scheme to a concept which is topmost in the broader/narrower concept hierarchies for that scheme, providing an entry point to these hierarchies.\n"@en .

skos:semanticRelation
        a                 rdf:Property , owl:ObjectProperty ;
        rdfs:domain       skos:Concept ;
        rdfs:isDefinedBy  <http://www.w3.org/2004/02/skos/core> ;
        rdfs:label        "is in semantic relation with"@en ;
        rdfs:range        skos:Concept ;
        skos:definition   "Links a concept to a concept related by meaning."@en ;
        skos:scopeNote    "\nThis property should not be used directly, but as a super-property for all properties denoting a relationship of meaning between concepts.\n"@en .

skos:OrderedCollection
        a                 owl:Class ;
        rdfs:isDefinedBy  <http://www.w3.org/2004/02/skos/core> ;
        rdfs:label        "Ordered Collection"@en ;
        rdfs:subClassOf   skos:Collection ;
        skos:definition   "\nAn ordered collection of concepts, where both the grouping and the ordering are meaningful.\n"@en ;
        skos:scopeNote    "\nOrdered collections can be used where you would like a set of concepts to be displayed in a specific order, and optionally under a 'node label'.\n"@en .

skos:hiddenLabel  a         rdf:Property , owl:AnnotationProperty ;
        rdfs:comment        "\nskos:prefLabel, skos:altLabel and skos:hiddenLabel are pairwise disjoint properties.\n"@en , "\nThe range of skos:hiddenLabel is the class of RDF plain literals.\n"@en ;
        rdfs:isDefinedBy    <http://www.w3.org/2004/02/skos/core> ;
        rdfs:label          "hidden label"@en ;
        rdfs:subPropertyOf  rdfs:label ;
        skos:definition     "\nA lexical label for a resource that should be hidden when generating visual displays of the resource, but should still be accessible to free text search operations.\n"@en .

<http://www.w3.org/2004/02/skos/core>
        a                owl:Ontology ;
        rdfs:seeAlso     <http://www.w3.org/TR/skos-reference/> ;
        dct:contributor  "\nParticipants in W3C's Semantic Web Deployment Working Group.\n" , "Nikki Rogers" , "Dave Beckett" ;
        dct:creator      "Sean Bechhofer" , "Alistair Miles" ;
        dct:description  "\nAn RDF vocabulary for describing the basic structure and content of concept schemes such as thesauri, classification schemes, subject heading lists, taxonomies, 'folksonomies', other types of controlled vocabulary, and also concept schemes embedded in glossaries and terminologies.\n"@en ;
        dct:title        "SKOS Vocabulary"@en .

skos:Collection  a        owl:Class ;
        rdfs:isDefinedBy  <http://www.w3.org/2004/02/skos/core> ;
        rdfs:label        "Collection"@en ;
        owl:disjointWith  skos:ConceptScheme , skos:Concept ;
        skos:definition   "A meaningful collection of concepts."@en ;
        skos:scopeNote    "\nLabelled collections can be used where you would like a set of concepts to be displayed under a 'node label' in the hierarchy.\n"@en .

skos:narrowMatch  a         rdf:Property , owl:ObjectProperty ;
        rdfs:isDefinedBy    <http://www.w3.org/2004/02/skos/core> ;
        rdfs:label          "has narrower match"@en ;
        rdfs:subPropertyOf  skos:narrower , skos:mappingRelation ;
        owl:inverseOf       skos:broadMatch ;
        skos:definition     "\nskos:narrowMatch is used to state a hierarchical mapping link between two conceptual resources in different concept schemes.\n"@en .

skos:note  a              rdf:Property , owl:AnnotationProperty ;
        rdfs:isDefinedBy  <http://www.w3.org/2004/02/skos/core> ;
        rdfs:label        "note"@en ;
        skos:definition   "A general note, for any purpose."@en ;
        skos:scopeNote    "\nThis property may be used directly, or as a super-property for more specific note types.\n"@en .

skos:narrower  a            rdf:Property , owl:ObjectProperty ;
        rdfs:comment        "\nNarrower concepts are typically rendered as children in a concept hierarchy (tree).\n"@en ;
        rdfs:isDefinedBy    <http://www.w3.org/2004/02/skos/core> ;
        rdfs:label          "has narrower"@en ;
        rdfs:subPropertyOf  skos:narrowerTransitive ;
        owl:inverseOf       skos:broader ;
        skos:definition     "\nRelates a concept to a concept that is more specific in meaning.\n"@en ;
        skos:scopeNote      "\nBy convention, skos:broader is only used to assert an immediate (i.e. direct) hierarchical link between two conceptual resources.\n"@en .